WebAssembly/Wasm_Ast.thy
@@ -8,6 +8,10 @@ type_synonym \<comment> \<open>static offset\<close>
   off = nat
 type_synonym \<comment> \<open>alignment exponent\<close>
   a = nat
+type_synonym \<comment> \<open>address\<close>
+  addr = nat
+type_synonym \<comment> \<open>timestamp\<close>
+  h = nat
 
 \<comment> \<open>primitive types\<close>
 typedecl i32
@@ -16,6 +20,7 @@ typedecl f32
 typedecl f64
 
 \<comment> \<open>memory\<close>
+\<comment> \<open>TODO: Use mt instead of nat?\<close>
 type_synonym byte = uint8
 
 typedef bytes = "UNIV :: (byte list) set" ..
@@ -39,8 +44,24 @@ lift_definition mem_append :: "mem \<Rightarrow> bytes \<Rightarrow> mem" is app
 typedecl host
 typedecl host_state
 
+datatype
+  sh = T_loc | T_sh
+
+datatype
+  ord = Unord | Seqcst
+
+datatype
+  tr = Anyref | Funcref
+
+record rt = \<comment> \<open>reference types\<close>
+  rt_sh :: sh
+  rt_tr :: tr
+
+datatype \<comment> \<open>numeric types\<close>
+  nt = T_i32 | T_i64 | T_f32 | T_f64
+
 datatype \<comment> \<open>value types\<close>
-  t = T_i32 | T_i64 | T_f32 | T_f64
+  t = Nt "nt" | Rt "rt"
 
 datatype \<comment> \<open>packed types\<close>
   tp = Tp_i8 | Tp_i16 | Tp_i32
@@ -49,19 +70,29 @@ datatype \<comment> \<open>mutability\<close>
   mut = T_immut | T_mut
 
 record tg = \<comment> \<open>global types\<close>
+  tg_sh :: sh
   tg_mut :: mut
   tg_t :: t
 
 datatype \<comment> \<open>function types\<close>
-  tf = Tf "t list" "t list" ("_ '_> _" 60)
+  tf = Tf "sh" "t list" "t list" ("_ _ '_> _" 60)
+
+record tt = \<comment> \<open>table types\<close>
+  tt_sh :: sh
+  tt_rt :: rt
+  tt_n :: "i option"
+
+record mt = \<comment> \<open>memory types\<close>
+  mt_sh :: sh
+  mt_n :: "i option"
 
 (* TYPING *)
 record t_context =
   types_t :: "tf list"
   func_t :: "tf list"
   global :: "tg list"
-  table :: "nat option"
-  memory :: "nat option"
+  table :: "tt"
+  memory :: "mt"
   local :: "t list"
   label :: "(t list) list"
   return :: "(t list) option"
@@ -69,8 +100,8 @@ record t_context =
 record s_context =
   s_inst :: "t_context list"
   s_funcs :: "tf list"
-  s_tab  :: "nat list"
-  s_mem  :: "nat list"
+  s_tab  :: "tt list"
+  s_mem  :: "mt list"
   s_globs :: "tg list"
 
 datatype
@@ -83,29 +114,57 @@ datatype
   unop_f = Neg | Abs | Ceil | Floor | Trunc | Nearest | Sqrt
 
 datatype
+  unop =
+    Unop_i unop_i
+    | Unop_f unop_f
+
+datatype
   binop_i = Add | Sub | Mul | Div sx | Rem sx | And | Or | Xor | Shl | Shr sx | Rotl | Rotr
 
 datatype
   binop_f = Addf | Subf | Mulf | Divf | Min | Max | Copysign
-  
+
+datatype
+  binop =
+    Binop_i t binop_i
+    | Binop_f t binop_f
+
 datatype
   testop = Eqz
-  
+
 datatype
   relop_i = Eq | Ne | Lt sx | Gt sx | Le sx | Ge sx
-  
+
 datatype
   relop_f = Eqf | Nef | Ltf | Gtf | Lef | Gef
-  
+
+datatype
+  relop =
+    Relop_i relop_i
+    | Relop_f relop_f
+
 datatype
   cvtop = Convert | Reinterpret
 
-datatype \<comment> \<open>values\<close>
-  v =
+datatype \<comment> \<open>numeric values\<close>
+  nv =
     ConstInt32 i32
     | ConstInt64 i64
     | ConstFloat32 f32
     | ConstFloat64 f64
+
+datatype \<comment> \<open>values\<close>
+  v =
+    NumVal nv
+    | NullRef
+    | Ref a
+
+record inst = \<comment> \<open>instances\<close>
+  types :: "tf list"
+  funcs :: "i list"
+  tab :: "i option"
+  mem :: "i option"
+  globs :: "i list"
 
 datatype \<comment> \<open>basic instructions\<close>
   b_e =
@@ -121,40 +180,41 @@ datatype \<comment> \<open>basic instructions\<close>
     | Br_table "i list" i
     | Return
     | Call i
-    | Call_indirect i
+    | Call_indirect ord i
     | Get_local i
     | Set_local i
     | Tee_local i
-    | Get_global i
-    | Set_global i
-    | Load t "(tp \<times> sx) option" a off
-    | Store t "tp option" a off
+    | Get_global ord i
+    | Set_global ord i
+    | Get_table ord
+    | Set_table ord
+    | Load t ord "(tp \<times> sx) option" a off
+    | Store t ord "tp option" a off
+    | Rmw t binop "(tp \<times> sx) option" a off
     | Current_memory
+    | Current_table
     | Grow_memory
+    | Grow_table
     | EConst v ("C _" 60)
-    | Unop_i t unop_i
-    | Unop_f t unop_f
-    | Binop_i t binop_i
-    | Binop_f t binop_f
+    | Unop unop
+    | Binop binop
     | Testop t testop
-    | Relop_i t relop_i
-    | Relop_f t relop_f
+    | Relop relop
     | Cvtop t cvtop t "sx option"
+    | Wait t
+    | Notify
+    | Fork i
+    | Instantiate inst
 
 datatype cl = \<comment> \<open>function closures\<close>
   Func_native i tf "t list" "b_e list"
 | Func_host tf host
 
-record inst = \<comment> \<open>instances\<close>
-  types :: "tf list"
-  funcs :: "i list"
-  tab :: "i option"
-  mem :: "i option"
-  globs :: "i list"
-
 type_synonym tabinst = "(cl option) list"
 
+\<comment> \<open>FIXME: Adding sh is right I think?\<close>
 record global =
+  g_sh :: sh
   g_mut :: mut
   g_val :: v
 
@@ -165,12 +225,27 @@ record s = \<comment> \<open>store\<close>
   mem :: "mem list"
   globs :: "global list"
 
+datatype fld = Val | Data | Elem | Length
+
+record reg = \<comment> \<open>region\<close>
+  Reg_addr :: addr
+  Reg_fld :: fld
+
+datatype l = \<comment> \<open>location\<close>
+  L_r reg
+  | L_ri reg i
+
 datatype e = \<comment> \<open>administrative instruction\<close>
   Basic b_e ("$_" 60)
   | Trap
   | Callcl cl
   | Label nat "e list" "e list"
   | Local nat i "v list" "e list"
+  | Ref addr
+  | Call_admin addr
+  | Fork_admin "e list"
+  | Wait_admin l nat
+  | Notify_admin l nat inst
 
 datatype Lholed =
     \<comment> \<open>L0 = v* [<hole>] e*\<close>
